

# DS 3001: Linear Models

$$\hat{y}_i = b_0 + b_1 z_{i1} + b_2 z_{i2}$$

$$\frac{1}{N} \sum_{i=1}^N z_{ij} = 0$$

1.1)

$$SSE = \sum_{i=1}^N (y_i - \hat{y}_i)^2$$

$$= \sum_{i=1}^N (y_i - (b_0 + b_1 z_{i1} + b_2 z_{i2}))^2$$

$$SSE = \sum_{i=1}^N (y_i - b_0 - b_1 z_{i1} - b_2 z_{i2})^2$$

1.2)

$$\frac{dSSE}{db_0} = \sum_{i=1}^N \frac{d}{db_0} (y_i - b_0 - b_1 z_{i1} - b_2 z_{i2})^2$$

$$= -2 \sum_{i=1}^N (y_i - b_0 - b_1 z_{i1} - b_2 z_{i2})$$

$$= -2 \sum_{i=1}^N e_i$$

$$\frac{dSSE}{db_1} = \sum_{i=1}^N \frac{d}{db_1} (y_i - b_0 - b_1 z_{i1} - b_2 z_{i2})^2$$

$$= -2 \sum_{i=1}^N z_{i1} (y_i - b_0 - b_1 z_{i1} - b_2 z_{i2})$$

$$= -2 \sum_{i=1}^N z_{i1} e_i$$

$$\frac{dSSE}{db_2} = \sum_{i=1}^N \frac{d}{db_2} (y_i - b_0 - b_1 z_{i1} - b_2 z_{i2})^2$$

$$= -2 \sum_{i=1}^N z_{i2} (y_i - b_0 - b_1 z_{i1} - b_2 z_{i2})$$

$$= -2 \sum_{i=1}^N z_{i2} e_i$$

1.3)

normal equations:  $\sum_{i=1}^N e_i = 0$ ,  $\sum_{i=1}^N e_i z_{i1} = 0$ ,  $\sum_{i=1}^N e_i z_{i2} = 0$

dividing by  $N$ ,  $\frac{1}{N} \sum_{i=1}^N e_i = 0$  average residual is zero.

other two equations:

$$\sum_{i=1}^N e_i z_{i1} = 0 \rightarrow e \cdot z_1 = 0, \sum_{i=1}^N e_i z_{i2} = 0 \rightarrow e \cdot z_2 = 0$$

residual vector is orthogonal, just like in single linear regression



1.4)

$b_0^* = \bar{y}$  ← optimal intercept

$$\sum_{i=1}^N e_i = 0$$

$$\sum_{i=1}^N (y_i - b_0 - b_1 z_{i1} - b_2 z_{i2}) = 0$$

$$\sum_{i=1}^N y_i - Nb_0 - b_1 \sum_{i=1}^N z_{i1} - b_2 \sum_{i=1}^N z_{i2} = 0$$

$$\sum_{i=1}^N z_{i1} = 0, \sum_{i=1}^N z_{i2} = 0 \leftarrow \text{because predictors are centered}$$

$$\sum_{i=1}^N y_i - Nb_0 = 0 \rightarrow \sum_{i=1}^N y_i = Nb_0$$

$$b_0^* = \frac{1}{N} \sum_{i=1}^N y_i = \bar{y} \leftarrow \text{optimal intercept is sample mean of } y$$

1.5)

$$A_b = C$$

$$\begin{bmatrix} \sum_{i=1}^N z_{i1}^2 & \sum_{i=1}^N z_{i1} z_{i2} \\ \sum_{i=1}^N z_{i1} z_{i2} & \sum_{i=1}^N z_{i2}^2 \end{bmatrix} \begin{bmatrix} b_1 \\ b_2 \end{bmatrix} = \begin{bmatrix} \sum_{i=1}^N z_{i1} (y_i - \bar{y}) \\ \sum_{i=1}^N z_{i2} (y_i - \bar{y}) \end{bmatrix}$$

$$1.6) z_{ij} = x_{ij} - m_j$$

$$\frac{1}{N} \begin{bmatrix} \sum_{i=1}^N z_{i1}^2 & \sum_{i=1}^N z_{i1} z_{i2} \\ \sum_{i=1}^N z_{i1} z_{i2} & \sum_{i=1}^N z_{i2}^2 \end{bmatrix} \begin{bmatrix} b_1 \\ b_2 \end{bmatrix} = \frac{1}{N} \begin{bmatrix} \sum_{i=1}^N z_{i1} (y_i - \bar{y}) \\ \sum_{i=1}^N z_{i2} (y_i - \bar{y}) \end{bmatrix}$$

following equation at top of question, we substitute and each entry of  $A/N$  is the covariance matrix of the original predictors.

For  $C$ ,

$$\frac{1}{N} \sum_{i=1}^N z_{i1} (y_i - \bar{y}) = \text{cov}(z_1, y) = \text{cov}(x_1, y)$$

is the vector of covariances between each predictor and response.

This tells us that intuitively, we're aligning the joint variability of the predictors with their joint variability with the outcome.